ind/DoublyLinkedListIface.fsti
@@ -77,7 +77,7 @@ val dll_head (d:pdll 'a) :
     (ensures (fun h0 n h1 ->
          B.modifies B.loc_none h0 h1 /\
          dll_valid h1 d /\
-         // node_valid h1 n /\ TODO: Need to prove this
+         node_valid h1 n /\
          as_list h0 d == as_list h1 d /\
          n == L.hd (as_list h0 d)))
 
@@ -87,7 +87,7 @@ val dll_tail (d:pdll 'a) :
     (ensures (fun h0 n h1 ->
          h0 == h1 /\
          dll_valid h1 d /\
-         // node_valid h1 n /\ TODO: Need to prove this
+         node_valid h1 n /\
          as_list h0 d == as_list h1 d /\
          n == snd (L.unsnoc (as_list h0 d))))
 
